src/lean4/human_eval/problem_163.lean
@@ -22,14 +22,20 @@ def problem_spec
 (impl: Nat → Nat → List Nat)
 -- inputs
 (a b : Nat) :=
+let isAscendingBy2 (r : List Nat) :=
+∀ i, i < r.length - 1 → r[i+1]! - r[i]! = 2
 -- spec
 let spec (result: List Nat) :=
-isEven result ∧ isAscending result ∧
+result.all (fun n => n % 2 = 0) ∧ isAscendingBy2 result ∧
+1 < result.length ∧
 let min_a_b := min a b;
 let max_a_b := max a b;
-min_a_b ≤ result[]
+if min_a_b = max_a_b ∧ 2 ∣ min_a_b
+then result = []
+else ((result[0]! = if 2 ∣ min_a_b then min_a_b else (min_a_b + 1)) ∧
+(result[result.length-1]! = if 2 ∣ max_a_b then max_a_b else max_a_b - 1))
 -- program terminates
-∃ result, impl string = result ∧
+∃ result, impl a b = result ∧
 -- return value satisfies spec
 spec result
 -- end_def problem_spec
@@ -37,9 +43,9 @@ spec result
 -- start_def generated_spec
 def generated_spec
 -- function signature
-(impl: String → String)
+(impl: Nat → Nat → List Nat)
 -- inputs
-(s : String) : Prop :=
+(a b : Nat) : Prop :=
 -- end_def generated_spec
 --start_def generated_spec_body
 sorry
@@ -48,15 +54,15 @@ sorry
 -- start_def spec_isomorphism
 theorem spec_isomorphism:
 ∀ impl,
-(∀ s, problem_spec impl s) ↔
-(∀ s, generated_spec impl s) :=
+(∀ a b, problem_spec impl a b) ↔
+(∀ a b, generated_spec impl a b) :=
 -- end_def spec_isomorphism
 -- start_def spec_isomorphism_proof
 sorry
 -- end_def spec_isomorphism_proof
 
 -- start_def implementation_signature
-def implementation (s: String) : String :=
+def implementation (a b: Nat) : List Nat :=
 -- end_def implementation_signature
 -- start_def implementation
 sorry
@@ -64,16 +70,16 @@ sorry
 
 -- Uncomment the following test cases after implementing the function
 -- start_def test_cases
--- #test implementation ([1, 2, 2, -4]: List Int) = (-9: Int)
--- #test implementation ([0, 1]: List Int) = (0: Int)
--- #test implementation ([]: List Int) = none
+-- #test implementation 2 8 = [2, 4, 6, 8]
+-- #test implementation 8 2 = [2, 4, 6, 8]
+-- #test implementation 10 14 = []
 -- end_def test_cases
 
 
 -- start_def correctness_definition
 theorem correctness
-(s: String)
-: problem_spec implementation s :=
+(a b: Nat)
+: problem_spec implementation a b :=
 -- end_def correctness_definition
 -- start_def correctness_proof
 sorry
