src/lean4/human_eval/problem_153.lean
@@ -18,10 +18,8 @@ docstring: |
     return 'Slices.SErviNGSliCes' since 'SErviNGSliCes' is the strongest extension
     (its strength is -1).
 test_cases:
-  - input: [[1,2,3,4,5,1], [1,2,3,4,2,-2]]
-    expected_output: [0,0,0,0,3,3]
-  - input: [[0,5,0,0,0,4], [4,1,1,0,0,-2]]
-    expected_output: [4,4,1,0,0,6]
+  - input: ['my_class', ['AA', 'Be', 'CC']]
+    expected_output: 'my_class.AA'
 -/
 -- end_def problem_details
 
@@ -87,9 +85,7 @@ sorry
 
 -- Uncomment the following test cases after implementing the function
 -- start_def test_cases
--- #test implementation ([1, 2, 2, -4]: List Int) = (-9: Int)
--- #test implementation ([0, 1]: List Int) = (0: Int)
--- #test implementation ([]: List Int) = none
+-- #test implementation 'my_class', ['AA', 'Be', 'CC'] = 'my_class.AA'
 -- end_def test_cases
 
 
