src/lean4/human_eval/problem_157.lean
@@ -25,9 +25,10 @@ def problem_spec
 -- spec
 let spec (result: Bool) :=
 result ↔
-  ((a * a + b * b = c * c) ∨
+  0 < a ∧ 0 < b ∧ 0 < c ∧
+  (((a * a + b * b = c * c) ∨
   (a * a + c * c = b * b) ∨
-  (b * b + c * c = a * a))
+  (b) * b + c * c = a * a))
 -- program terminates
 ∃ result, impl a b c = result ∧
 -- return value satisfies spec
